@@ -1,0 +1,225 @@
+From stdpp Require Import list. 
+From TensorRocq Require Export Monoid.
+From TensorRocq Require Import AbstractTensorQuote.
+From TensorRocq Require Import Aux_relset.
+
+(* FIXME: Move *)
+
+Lemma foldr_assoc_to_unit {A} {R : relation A} `{!Equivalence R}
+  (e : A) (op : A -> A -> A)
+  `{opP : !Proper (R ==> R ==> R) op, ope : !LeftId R e op, opA : !Assoc R op}
+  (a : A) (l : list A) :
+  R (foldr op a l) (op (foldr op e l) a).
+Proof.
+  induction l.
+  - cbn.
+    now rewrite (left_id _ _).
+  - cbn.
+    rewrite IHl.
+    apply opA.
+Qed.
+
+Lemma foldr_app_assoc {A} {R : relation A} `{!Equivalence R}
+  (e : A) (op : A -> A -> A)
+  `{opP : !Proper (R ==> R ==> R) op, ope : !LeftId R e op, opA : !Assoc R op}
+  (l l' : list A) :
+  R (foldr op e (l ++ l')) (op (foldr op e l) (foldr op e l')).
+Proof.
+  rewrite foldr_app.
+  now apply foldr_assoc_to_unit.
+Qed.
+
+
+
+
+(* FIXME: Move, or maybe it exists already? *)
+Inductive btree {A : Type} : Type :=
+  | bnode : btree -> btree -> btree
+  | bleaf : A -> btree
+  | bempty : btree.
+#[global] Arguments btree (A) : clear implicits.
+
+#[export] Instance btree_empty A : Empty (btree A) := bempty.
+
+Fixpoint btree_fold {A B} (e : B) (ofa : A -> B)
+  (op : B -> B -> B) (t : btree A) : B :=
+  match t with
+  | bnode l r => op (btree_fold e ofa op l) (btree_fold e ofa op r)
+  | bleaf a => ofa a
+  | bempty => e
+  end.
+
+Fixpoint btree_elems {A} (t : btree A) : list A :=
+  match t with
+  | bnode l r => btree_elems l ++ btree_elems r
+  | bleaf a => [ a ]
+  | bempty => []
+  end.
+
+Coercion btree_elems : btree >-> list.
+
+#[export] Instance btree_equiv A : Equiv (btree A) :=
+  fun t t' => btree_elems t = btree_elems t'.
+
+
+
+Lemma btree_fold_to_list {A B} (e : B) (ofa : A -> B)
+  (op : B -> B -> B) `{R : relation B, HR : !Equivalence R}
+  `{eop : !LeftId R e op, ope : !RightId R e op, opa : !Assoc R op,
+  opP : !Proper (R ==> R ==> R) op}
+  bw : R (btree_fold e ofa op bw) (foldr op e (ofa <$> btree_elems bw)).
+Proof.
+  induction bw.
+  - cbn.
+    rewrite fmap_app.
+    rewrite (foldr_app_assoc _ _ _).
+    now f_equiv.
+  - cbn.
+    now rewrite (right_id _ _).
+  - done.
+Qed.
+
+#[export] Instance btree_fold_Proper {A B} (e : B) (ofa : A -> B)
+  (op : B -> B -> B) `{R : relation B, HR : !Equivalence R}
+  `{eop : !LeftId R e op, ope : !RightId R e op, opa : !Assoc R op,
+  opP : !Proper (R ==> R ==> R) op} :
+  Proper (equiv ==> R) (btree_fold e ofa op).
+Proof.
+  intros bw bw' [= Hbw].
+  rewrite 2 (btree_fold_to_list _ _ _).
+  now rewrite Hbw.
+Qed.
+
+#[export] Instance btree_monoid A :
+  Monoid (btree A) ∅ bnode equiv.
+Proof.
+  split.
+  - apply _.
+  - intros x x' Hx y y' Hy.
+    hnf.
+    cbn.
+    now f_equal.
+  - intros x y z.
+    hnf.
+    cbn.
+    apply app_assoc.
+  - easy.
+  - intros x.
+    hnf.
+    cbn.
+    apply app_nil_r.
+Qed.
+
+#[refine] Instance btree_free_monoid A :
+  FreeMonoid (btree A) A := {
+  mdecomp b := b;
+  mdecomp_inv a := bleaf a;
+}.
+Proof.
+  - abstract easy.
+  - abstract easy.
+  - abstract easy.
+  - abstract easy.
+Defined.
+
+
+
+
+
+
+
+
+
+
+
+
+
+
+
+
+
+
+
+
+
+
+
+
+
+
+Class QuoteMonoidSize {M} (f : M -> nat)
+  `{MD : Monoid M mO madd meq, MS : !MonoidSize f}
+  (a : M) (n : nat) := {
+  quote_msize : f a = n
+}.
+
+#[global] Hint Mode QuoteMonoidSize + ! + + + + ! - + : typeclass_instances.
+
+
+
+Section BWQuotation.
+
+
+#[local] Set Typeclasses Unique Instances.
+
+Definition denote_nat_bw (l : list nat) (bw : btree (option nat)) : nat :=
+  btree_fold 0 (λ k, from_option (default 0 ∘ (l !!.)) 1 k) Nat.add bw.
+
+#[global] Instance denote_nat_bw_MonoidSize {l : list nat} :
+  MonoidSize (denote_nat_bw l).
+Proof.
+  split.
+  - apply btree_fold_Proper; apply _.
+  - done.
+  - done.
+Qed.
+
+#[export] Instance quote_denote_nat_bw_0 (l : list nat) :
+  QuoteMonoidSize (denote_nat_bw l) bempty 0.
+Proof.
+  now constructor.
+Qed.
+
+#[export] Instance quote_denote_nat_bw_S (l : list nat) bw n :
+  QuoteMonoidSize (denote_nat_bw l) bw n ->
+  QuoteMonoidSize (denote_nat_bw l) (bnode (bleaf None) bw) (S n).
+Proof.
+  intros [Hbw].
+  constructor.
+  now rewrite <- Hbw.
+Qed.
+
+(* Small optimization *)
+#[export] Instance quote_denote_nat_bw_1 (l : list nat) :
+  QuoteMonoidSize (denote_nat_bw l) (bleaf None) 1.
+Proof.
+  now constructor.
+Qed.
+
+
+#[export] Instance quote_denote_nat_bw_add (l : list nat) bw bw' n m :
+  QuoteMonoidSize (denote_nat_bw l) bw n ->
+  QuoteMonoidSize (denote_nat_bw l) bw' m ->
+  QuoteMonoidSize (denote_nat_bw l) (bnode bw bw') (n + m).
+Proof.
+  intros [Hbw] [Hbw'].
+  constructor.
+  now rewrite <- Hbw, <- Hbw'.
+Qed.
+
+(* TODO: Maybe replace with lemma and hint extern? My concern is that the
+  hint extern may not do the same reduction/unification as TC generally,
+  so this may be (ironically) overapplied in that case *)
+#[export] Instance quote_denote_nat_bw_const (l : list nat) n k :
+  IsNth n k l ->
+  QuoteMonoidSize (denote_nat_bw l) (bleaf (Some k)) n | 10.
+Proof.
+  intros Hnth%IsNth_iff.
+  constructor.
+  cbn.
+  now rewrite Hnth.
+Qed.
+
+
+
+End BWQuotation.
